Clean up fuel-less parser implementation, add proof automation

LL1/Parser.v
@@ -1,8 +1,9 @@
-Require Import FMaps List MSets String Program.Wf Arith.Wf_nat.
+Require Import FMaps List MSets Omega String Program.Wf Arith.Wf_nat.
 Require Import Lib.Grammar.
 Require Import Lib.ParseTree.
 Require Import Lib.Utils.
 Require Import Lib.Tactics.
+Require Import LL1.Derivation.
 Require Import LL1.ParseTable. 
 Require Import LL1.ParseTableGen. (* for fromNtList *)
 Import ListNotations.
@@ -157,104 +158,17 @@ Section TripleLT.
     inv H; eauto.
   Defined.
 
-  Definition bool_order (b1 b2 : bool) : Prop :=
-    b1 = false /\ b2 = true.
-
-  Theorem bool_order_trans : transitive _ bool_order.
-  Proof.
-    intros x y z Hxy Hyz.
-    inv Hxy; inv Hyz; congruence.
-  Defined.
-  
-  Theorem bool_order_wf : well_founded bool_order.
-  Proof.
-    intros b2.
-    constructor.
-    intros b1 Hbo.
-    inv Hbo.
-    constructor.
-    intros b1 Hbo.
-    inv Hbo.
-    congruence.
-  Defined.
-
 End TripleLT.
-
-Section PairLT.
-
-  Variables (A B : Type) (ltA : relation A) (ltB : relation B).
-
-  Inductive pair_lex : A * B -> A * B -> Prop :=
-  | pr_fst_lt : forall x x' y y', ltA x x' -> pair_lex (x, y) (x', y')
-  | pr_snd_lt : forall x y y', ltB y y' -> pair_lex (x, y) (x, y').
-
-  Hint Constructors pair_lex.
-
-  Theorem pair_lex_trans :
-    transitive _ ltA -> transitive _ ltB -> transitive _ pair_lex.
-  Proof.
-    intros tA tB [x1 y1] [x2 y2] [x3 y3] H12 H23.
-    inv H12; inv H23; eauto.
-  Defined.
-
-  Theorem pair_lex_wf :
-    well_founded ltA -> well_founded ltB -> well_founded pair_lex.
-  Proof.
-    intros wfA wfB [x y].
-    revert y.
-    induction (wfA x) as [x _ IHx].
-    intros y.
-    induction (wfB y) as [y _ IHy].
-    constructor.
-    intros [x' y'] H.
-    inv H; eauto.
-  Defined.
-
-End PairLT.
-
-Set Implicit Arguments.
-
-Definition triple_lt : relation (nat * nat * bool) :=
-  triple_lex nat nat bool lt lt bool_order.
-
-Definition triple_lt_ind :=
-  triple_lex_ind nat nat bool lt lt bool_order.
-
-Lemma triple_lt_wf :
-  well_founded triple_lt.
-Proof.
-  apply triple_lex_wf.
-  - apply lt_wf.
-  - apply lt_wf.
-  - apply bool_order_wf.
-Defined.
 
 Inductive sym_arg : Set :=
 | F_arg : symbol -> sym_arg
 | G_arg : list symbol -> sym_arg.
-
-Definition boolOf (sa : sym_arg) : bool :=
-  match sa with
-  | F_arg _ => false
-  | G_arg _ => true
-  end.
 
 Definition nt_keys (tbl : parse_table) : list nonterminal :=
   List.map (fun pr => match pr with 
                       | ((x, _), _) => x
                       end)
            (ParseTable.elements tbl).
-
-Definition meas (tbl : parse_table) (triple : list string * list nonterminal * sym_arg) : nat * nat * bool :=
-  match triple with
-  | (word, visited, sa) =>
-    (List.length word,
-     NtSet.cardinal (NtSet.diff (fromNtList (nt_keys tbl)) (fromNtList visited)),
-     boolOf sa)
-  end.
-
-Definition triple_le (tr1 tr2 : nat * nat * bool) : Prop :=
-  triple_lt tr1 tr2 \/ tr1 = tr2.
 
 Lemma not_in_list_iff_not_in_fromNtList:
   forall (x : NtSet.elt) (l : list NtSet.elt),
@@ -273,49 +187,6 @@ Proof.
   apply Nat_as_DT.lt_trans.
 Defined.
 
-Lemma triple_lt_le_trans :
-  forall (x y z : nat * nat * bool),
-    triple_lt x y
-    -> triple_le y z
-    -> triple_lt x z.
-Proof.
-  intros x y z Hlt Hle.
-  destruct Hle.
-  - eapply triple_lex_trans; eauto.
-    + apply lt_trans.
-    + apply lt_trans.
-    + apply bool_order_trans.
-  - subst; auto.
-Defined.
-
-Lemma triple_le_lt_trans :
-  forall (x y z : nat * nat * bool),
-    triple_le x y
-    -> triple_lt y z
-    -> triple_lt x z.
-Proof.
-  intros x y z Hle Hlt.
-  destruct Hle.
-  - eapply triple_lex_trans; eauto.
-    + apply lt_trans.
-    + apply lt_trans.
-    + apply bool_order_trans.
-  - subst; auto.
-Defined.
-
-Lemma triple_lt_trans :
-  forall (x y z : nat * nat * bool),
-    triple_lt x y
-    -> triple_lt y z
-    -> triple_lt x z.
-Proof.
-  intros x y z Hxy Hyz.
-  eapply triple_lex_trans; eauto.
-  - apply lt_trans.
-  - apply lt_trans.
-  - apply bool_order_trans.
-Defined.
-
 Lemma pt_lookup_in_nt_keys :
   forall x la tbl gamma,
     pt_lookup x la tbl = Some gamma
@@ -332,357 +203,6 @@ Proof.
     + right; auto.
 Defined.
         
-(* Fuel-less LL(1) parser defined with Program Fixpoint,
-   termination proof handled separately from function definition *)
-Program Fixpoint parse1 (tbl     : parse_table)
-                        (tri     : list string * list nonterminal * sym_arg)
-                        {measure (meas tbl tri) (triple_lt)}
-                        : sum parse_failure
-                              (sum (list tree * {tri' | triple_le (meas tbl tri') (meas tbl tri)})
-                                   (tree      * {tri' | triple_lt (meas tbl tri') (meas tbl tri)})) :=
-  match tri with
-  | (word, vis, sa) =>
-    match sa with
-    | F_arg sym =>
-      (* morally, a call to parse *)
-      match (sym, word) with
-      | (T y, nil) => inl (Mismatch "error message" word)
-      | (T y, token :: word') =>
-        if beqString y token then
-          inr (inr (Leaf y, (word', nil, sa)))
-        else
-          inl (Mismatch "error message" word)
-      | (NT x, _) =>
-        if List.in_dec NT_as_DT.eq_dec x vis then
-          inl (LeftRec (x :: vis))
-        else
-          match pt_lookup x (peek word) tbl with
-          | None => inl (Mismatch "error message" word)
-          | Some gamma =>
-            match parse1 tbl (word, x :: vis, G_arg gamma) with
-            | inl pf => inl pf
-            | inr (inr (_, _)) => inl Error
-            | inr (inl (sts, exist _ tri' _)) => inr (inr (Node x sts, exist _ tri' _))
-            end
-          end
-      end
-    | G_arg gamma =>
-      (* a call to parseForest *)
-      match gamma with
-      | nil => inr (inl (nil, (word, vis, sa)))
-      | sym :: gamma' =>
-        match parse1 tbl (word, vis, F_arg sym) with
-        | inl pf => inl pf
-        | inr (inl (_, _)) => inl Error
-        | inr (inr (lSib, exist _ tri' _)) =>
-          match parse1 tbl tri' with
-          | inl pf => inl pf
-          | inr (inr (_, _)) => inl Error
-          | inr (inl (rSibs, exist _ tri'' _)) =>
-            inr (inl (lSib :: rSibs, exist _ tri'' _))
-          end
-        end
-      end
-    end
-  end.
-Obligation 1.
-apply fst_lt; auto.
-Defined.
-Obligation 2.
-simpl.
-apply snd_lt.
-apply NP.subset_cardinal_lt with (x := x).
-- ND.fsetdec. 
-- apply in_A_not_in_B_in_diff.
-  + apply in_list_iff_in_fromNtList.
-    eapply pt_lookup_in_nt_keys; eauto.
-  + apply not_in_list_iff_not_in_fromNtList; auto.
-- ND.fsetdec.
-Defined.
-Obligation 3.
-destruct Heq_tri.
-eapply triple_le_lt_trans; eauto.
-apply snd_lt.
-apply NP.subset_cardinal_lt with (x := x).
-- ND.fsetdec. 
-- apply in_A_not_in_B_in_diff.
-  + apply in_list_iff_in_fromNtList.
-    eapply pt_lookup_in_nt_keys; eauto.
-  + apply not_in_list_iff_not_in_fromNtList; auto.
-- ND.fsetdec.
-Defined.
-Obligation 4.
-red; auto.
-Defined.
-Obligation 5.
-apply thd_lt; red; auto.
-Defined.
-Obligation 6.
-destruct Heq_tri.
-simpl.
-eapply triple_lt_trans; eauto.
-apply thd_lt; red; auto.
-Defined.
-Obligation 7.
-(* there might be a shorter proof for this one *)
-destruct Heq_tri.
-left.
-eapply triple_le_lt_trans; eauto.
-eapply triple_lt_trans; eauto.
-apply thd_lt; red; auto.
-Defined.
-Obligation 8.
-apply measure_wf.
-apply triple_lex_wf.
-- apply lt_wf.
-- apply lt_wf.
-- apply bool_order_wf.
-Defined.
-
-(* Plan :
-   - replace obligations with proof terms (* done! *)
-   - add Acc arg  (* done! *)
-   - replace refine-generated termination proofs with lemmas (* done! *)
-   - see if Function can generate correct rewriting lemma (* done -- it can't *)
-   - switch to two mutually recursive functions *)
-
-Lemma tail_lt_word :
-  forall tbl tri word token word' vis vis' sa sa',
-    tri = (word, vis, sa)
-    -> word = token :: word'
-    -> triple_lt (meas tbl (word', vis', sa')) (meas tbl tri).
-Proof.
-  intros.
-  subst.
-  apply fst_lt; auto.
-Defined.
-
-Lemma vis_lt_add :
-  forall tbl (tri tri' : list string * list nonterminal * sym_arg) word vis sa sa' x gamma,
-    tri = (word, vis, sa)
-    -> ~ In x vis
-    -> pt_lookup x (peek word) tbl = Some gamma
-    -> triple_le (meas tbl tri') (meas tbl (word, x :: vis, sa'))
-    -> triple_lt (meas tbl tri') (meas tbl tri).
-Proof.
-  intros; subst.
-  eapply triple_le_lt_trans; eauto.
-  apply snd_lt; simpl.
-  apply NP.subset_cardinal_lt with (x := x).
-  - ND.fsetdec. 
-  - apply in_A_not_in_B_in_diff.
-    + apply in_list_iff_in_fromNtList.
-      eapply pt_lookup_in_nt_keys; eauto.
-    + apply not_in_list_iff_not_in_fromNtList; auto.
-  - ND.fsetdec.
-Defined.
-
-Lemma triple_le_refl :
-  forall tbl tri word vis sa,
-    tri = (word, vis, sa)
-    -> triple_le (meas tbl (word, vis, sa)) (meas tbl tri).
-Proof.
-  intros; subst.
-  right; auto.
-Defined.
-
-Lemma pf_lt_args :
-  forall tbl tri tri' tri'' word vis sa gamma sym gamma',
-    tri = (word, vis, sa)
-    -> sa = G_arg gamma
-    -> gamma = sym :: gamma'
-    -> triple_lt (meas tbl tri') (meas tbl (word, vis, F_arg sym))
-    -> triple_le (meas tbl tri'') (meas tbl tri')
-    -> triple_le (meas tbl tri'') (meas tbl tri).
-Proof.
-  intros; subst.
-  left.
-  eapply triple_le_lt_trans; eauto.
-  eapply triple_lt_trans; eauto.
-  apply thd_lt; red; auto.
-Defined.
-
-Lemma acc_vis_add :
-  forall tbl tri word vis sa sym x gamma,
-    tri = (word, vis, sa)
-    -> sa = F_arg sym
-    -> ~ In x vis
-    -> pt_lookup x (peek word) tbl = Some gamma
-    -> Acc triple_lt (meas tbl tri)
-    -> Acc triple_lt (meas tbl (word, x :: vis, G_arg gamma)).
-Proof.
-  intros; subst; simpl.
-  eapply Acc_inv; eauto.
-  apply snd_lt.
-  apply NP.subset_cardinal_lt with (x := x).
-  - ND.fsetdec.
-  - apply in_A_not_in_B_in_diff.
-    + apply in_list_iff_in_fromNtList.
-      eapply pt_lookup_in_nt_keys; eauto.
-    + apply not_in_list_iff_not_in_fromNtList; auto.
-  - ND.fsetdec.
-Defined.
-
-(* to do : more hypotheses than needed, probably *)
-Lemma if_acc_gamma_then_acc_sym :
-  forall tbl tri word vis sa gamma sym gamma',
-    Acc triple_lt (meas tbl tri)
-    -> tri = (word, vis, sa)
-    -> sa = G_arg gamma
-    -> gamma = sym :: gamma'
-    -> Acc triple_lt (meas tbl (word, vis, F_arg sym)).
-Proof.
-  intros; subst; simpl.
-  eapply Acc_inv; eauto.
-  apply thd_lt.
-  red; eauto.
-Defined.
-
-Lemma acc_triple_lt_trans :
-  forall tbl tri word vis sa gamma sym gamma' tri',
-  Acc triple_lt (meas tbl tri)
-  -> tri = (word, vis, sa)
-  -> sa = G_arg gamma
-  -> gamma = sym :: gamma'
-  -> triple_lt (meas tbl tri') (meas tbl (word, vis, F_arg sym))
-  -> Acc triple_lt (meas tbl tri').
-Proof.
-  intros; subst; simpl in *.
-  eapply Acc_inv; eauto.
-  eapply triple_lt_trans; eauto.
-  apply thd_lt.
-  red; auto.
-Defined.
-
-(* Fuel-less LL(1) parser defined with refine instead of Program Fixpoint,
-   termination proof handled separately from function definition *)
-Fixpoint parse2 (tbl     : parse_table)
-         (tri     : list string * list nonterminal * sym_arg)
-         (a : Acc triple_lt (meas tbl tri))
-         {struct a}
-  : sum parse_failure
-        (sum (list tree * {tri' | triple_le (meas tbl tri') (meas tbl tri)})
-             (tree      * {tri' | triple_lt (meas tbl tri') (meas tbl tri)})).
-  refine (match tri as tri' return tri = tri' -> _ with
-          | (word, vis, sa) =>
-            fun Htri => match sa as sa' return sa = sa' -> _ with
-                        | F_arg sym =>
-                          (* morally, a call to parse *)
-                          fun Hsa => match sym with
-                                   | T y  => match word as w return word = w -> _ with
-                                             | [] => fun _ => inl (Mismatch "error message" word)
-                                             | token :: word' =>
-                                               if beqString y token then
-                                                 fun Hword =>
-                                                   inr (inr (Leaf y, exist _ (word', nil, sa) _))
-                                               else
-                                                 fun _ => inl (Mismatch "error message" word)
-                                             end eq_refl
-                                   | NT x =>
-                                     match List.in_dec NT_as_DT.eq_dec x vis with
-                                     | left _ => inl (LeftRec (x :: vis))
-                                     | right Hnin => 
-                                       match pt_lookup x (peek word) tbl as H return  pt_lookup x (peek word) tbl = H -> _ with
-                                       | None => fun _ => inl (Mismatch "error message" word)
-                                       | Some gamma =>
-                                         fun Hlk => match parse2 tbl (word, x :: vis, G_arg gamma) _ with
-                                                    | inl pf => inl pf
-                                                    | inr (inr (_, _)) => inl Error
-                                                    | inr (inl (sts, exist _ tri' Htri')) =>
-                                                      inr (inr (Node x sts, exist _ tri' _))
-                                                    end
-                                       end eq_refl
-                                     end
-                                   end
-                        | G_arg gamma =>
-                          (* a call to parseForest *)
-                          fun Hsa => match gamma as g return gamma = g -> _ with
-                                     | nil =>
-                                       fun _ => inr (inl (nil, exist _ (word, vis, sa) _))
-                                     | sym :: gamma' =>
-                                       fun Hgamma => match parse2 tbl (word, vis, F_arg sym) _ with
-                                                     | inl pf => inl pf
-                                                     | inr (inl (_, _)) => inl Error
-                                                     | inr (inr (lSib, exist _ tri' Htri')) =>
-                                                       match parse2 tbl tri' _ with
-                                                       | inl pf => inl pf
-                                                       | inr (inr (_, _)) => inl Error
-                                                       | inr (inl (rSibs, exist _ tri'' Htri'')) =>
-                                                         inr (inl (lSib :: rSibs, exist _ tri'' _))
-                                                       end
-                                                     end
-                                     end eq_refl
-                        end eq_refl
-          end eq_refl).
-  - eapply tail_lt_word; eauto.
-  - eapply acc_vis_add; eauto.
-  - apply (vis_lt_add tri' Htri Hnin Hlk Htri').
-  - eapply triple_le_refl; eauto.
-  - eapply if_acc_gamma_then_acc_sym; eauto.
-  - eapply acc_triple_lt_trans; eauto.
-  - eapply (pf_lt_args _ _ Htri Hsa Hgamma Htri' Htri''); eauto.
-Defined.
-  
-(* Fuel-less LL(1) parser with termination proof "inlined" *)
-Fixpoint parse3 (tbl     : parse_table)
-         (tri     : list string * list nonterminal * sym_arg)
-         (a : Acc triple_lt (meas tbl tri))
-         {struct a}
-  : sum parse_failure
-        (sum (list tree * {tri' | triple_le (meas tbl tri') (meas tbl tri)})
-             (tree      * {tri' | triple_lt (meas tbl tri') (meas tbl tri)})) :=
-  match tri as tri' return tri = tri' -> _ with
-  | (word, vis, sa) =>
-    fun Htri => match sa as sa' return sa = sa' -> _ with
-                | F_arg sym =>
-                  (* morally, a call to parse *)
-                  fun Hsa => match sym with
-                             | T y  => match word as w return word = w -> _ with
-                                       | [] => fun _ => inl (Mismatch "error message" word)
-                                       | token :: word' =>
-                                         if beqString y token then
-                                           fun Hword =>
-                                             inr (inr (Leaf y, exist _ (word', nil, sa) (tail_lt_word tbl _ _ Htri Hword)))
-                                         else
-                                           fun _ => inl (Mismatch "error message" word)
-                                       end (eq_refl _)
-                             | NT x =>
-                               match List.in_dec NT_as_DT.eq_dec x vis with
-                               | left _ => inl (LeftRec (x :: vis))
-                               | right Hnin => 
-                                 match pt_lookup x (peek word) tbl as H return  pt_lookup x (peek word) tbl = H -> _ with
-                                 | None => fun _ => inl (Mismatch "error message" word)
-                                 | Some gamma =>
-                                   fun Hlk => match parse3 tbl (word, x :: vis, G_arg gamma) (acc_vis_add tbl x Htri Hsa Hnin Hlk a) with
-                                              | inl pf => inl pf
-                                              | inr (inr (_, _)) => inl Error
-                                              | inr (inl (sts, exist _ tri' Htri')) =>
-                                                inr (inr (Node x sts, exist _ tri' (vis_lt_add tri' Htri Hnin Hlk Htri')))
-                                              end
-                                 end (eq_refl _)
-                               end
-                             end
-                | G_arg gamma =>
-                  (* a call to parseForest *)
-                  fun Hsa => match gamma as g return gamma = g -> _ with
-                             | nil =>
-                               fun _ => inr (inl (nil, exist _ (word, vis, sa) (triple_le_refl tbl Htri)))
-                             | sym :: gamma' =>
-                               fun Hgamma => match parse3 tbl (word, vis, F_arg sym) (if_acc_gamma_then_acc_sym tbl a Htri Hsa Hgamma) with
-                                             | inl pf => inl pf
-                                             | inr (inl (_, _)) => inl Error
-                                             | inr (inr (lSib, exist _ tri' Htri')) =>
-                                               match parse3 tbl tri' (acc_triple_lt_trans tri' a Htri Hsa Hgamma Htri') with
-                                               | inl pf => inl pf
-                                               | inr (inr (_, _)) => inl Error
-                                               | inr (inl (rSibs, exist _ tri'' Htri'')) =>
-                                                 inr (inl (lSib :: rSibs, exist _ tri'' (pf_lt_args _ _ Htri Hsa Hgamma Htri' Htri'')))
-                                               end
-                                             end
-                             end (eq_refl _)
-                end (eq_refl _)
-  end (eq_refl _).
-
 Definition ptlk_dec x la tbl : sum (pt_lookup x la tbl = None) {gamma | pt_lookup x la tbl = Some gamma}.
   destruct (pt_lookup x la tbl) eqn:Hlk.
   - right.
@@ -690,939 +210,6 @@ Definition ptlk_dec x la tbl : sum (pt_lookup x la tbl = None) {gamma | pt_looku
   - left.
     auto.
 Defined.
-    
-Fixpoint parse4 (tbl     : parse_table)
-         (word : list string)
-         (vis : list nonterminal)
-         (sa : sym_arg)
-         (a       : Acc triple_lt (meas tbl (word, vis, sa)))
-         {struct a}
-  : sum parse_failure
-        (sum (list tree * {tri' | triple_le (meas tbl tri') (meas tbl (word, vis, sa))})
-             (tree      * {tri' | triple_lt (meas tbl tri') (meas tbl (word, vis, sa))})).
-  refine (match sa as sa' return sa = sa' -> _ with
-          | F_arg sym =>
-            fun Hsa => match sym with
-                       | T y  => match word as w return word = w -> _ with
-                                 | [] => fun _ => inl (Mismatch "error message" word)
-                                 | token :: word' =>
-                                   if beqString y token then
-                                     fun Hword =>
-                                       inr (inr (Leaf y, exist _ (word', nil, sa) _))
-                                   else
-                                     fun _ => inl (Mismatch "error message" word)
-                                 end eq_refl
-                       | NT x =>
-                         match List.in_dec NT_as_DT.eq_dec x vis with
-                         | left _ => inl (LeftRec (x :: vis))
-                         | right Hnin =>
-                           match ptlk_dec x (peek word) tbl with
-                           | inl _ => inl (Mismatch "error message" word)
-                           | inr (exist _ gamma Hlk) =>
-                           (*match pt_lookup x (peek word) tbl as H return pt_lookup x (peek word) tbl = H -> _ with
-                           | None => fun _ => inl (Mismatch "error message" word)
-                           | Some gamma => *)
-                             match parse4 tbl word (x :: vis) (G_arg gamma) _ with (*word (x :: vis) (G_arg gamma) a with *)
-                                        | inl pf => inl pf
-                                        | inr (inr _) => inl Error
-                                        | inr (inl (sts, exist _ tri' Htri')) =>
-                                          inr (inr (Node x sts, exist _ tri' _))
-                                        end
-                           end
-                         end
-                       end
-          | G_arg gamma =>
-            fun Hsa => match gamma as g return gamma = g -> _ with
-                       | nil =>
-                         fun _ => inr (inl (nil, exist _ (word, vis, sa) _))
-                       | sym :: gamma' =>
-                         fun Hgamma => match parse4 tbl word vis (F_arg sym) _ with (* tbl word vis F_arg sym (if_acc_gamma_then_acc_sym tbl a _ Hsa Hgamma) with *)
-                                       | inl pf => inl pf
-                                       | inr (inl _) => inl Error
-                                       | inr (inr (lSib, exist _ tri' Htri')) =>
-                                         match tri' as tri'2 return tri' = tri'2 -> _ with
-                                         | (word', vis', _) =>
-                                           fun Htri'eq => match parse4 tbl word' vis' (G_arg gamma') _ with (* tbl word' vis' (G_arg gamma') (acc_triple_lt_trans _ a _ Hsa Hgamma Htri') with*)
-                                                          | inl pf => inl pf
-                                                          | inr (inr _) => inl Error
-                                                          | inr (inl (rSibs, exist _ tri'' Htri'')) =>
-                                                            inr (inl (lSib :: rSibs, exist _ tri'' _))
-                                                          end
-                                         end eq_refl
-                                       end
-                       end eq_refl
-          end eq_refl).
-  - eapply tail_lt_word; eauto.
-  - eapply acc_vis_add; eauto.
-  - eapply vis_lt_add; eauto.
-  - eapply triple_le_refl; eauto.
-  - eapply if_acc_gamma_then_acc_sym; eauto.
-  - subst.
-    inv Htri'.
-    + eapply Acc_inv; eauto.
-      apply fst_lt; auto.
-    + simpl.
-      subst.
-      eapply Acc_inv; eauto.
-      simpl.
-      rewrite H3.
-      apply snd_lt; auto.
-    + inv H0.
-      congruence.
-  - subst.
-    inv Htri'.
-    + eapply pf_lt_args; eauto.
-      apply fst_lt; auto.
-    + eapply pf_lt_args; eauto.
-      simpl.
-      rewrite H3.
-      apply snd_lt; auto.
-    + inv H0.
-      congruence.
-Defined.
-
-Definition isLeft (A B : Type) (e : sum A B) : bool :=
-  match e with
-  | inl _ => true
-  | inr _ => false
-  end.
-
-Definition isRight (A B : Type) (e : sum A B) : bool :=
-  negb (isLeft e).
-
-Lemma sym_ret_inr :
-  forall (tbl : parse_table)
-         (word : list string)
-         (vis : list nonterminal)
-         (sa : sym_arg)
-         e,
-    parse4 (triple_lt_wf (meas tbl (word, vis, sa))) = inr e
-    -> forall (sym : symbol),
-      sa = F_arg sym
-      -> isRight e = true.
-Proof.
-  intros; subst; simpl in *.
-  destruct sym.
-  - destruct word.
-    + congruence.
-    + destruct (beqString t s) eqn:Hbeq.
-      * inv H.
-        auto.
-      * inv H.
-  - destruct (in_dec ND.F.eq_dec n vis).
-    + inv H.
-    + destruct (ptlk_dec n (peek word) tbl). 
-      * congruence.
-      * destruct s as [gamma Hlk].
-        repeat match goal with
-               | H : context[match ?X with
-                             | _ => _
-                             end] |- _ =>
-                 destruct X
-               end.
-        -- congruence.
-        -- inv H.
-           auto.
-        -- congruence.
-Qed.
-  (* Alright! We're able to simplify a parser application in a proof setting *)
-
-(* Goal: lemma-tize the previous function so that I can inline the termination proofs *)
-
-Lemma hole1 :
-  forall tbl token word' vis vis' sa sa',
-    triple_lt (meas tbl (word', vis', sa')) (meas tbl (token :: word', vis, sa)).
-Proof.
-  intros.
-  apply fst_lt.
-  auto.
-Defined.
-
-Lemma hole2 :
-  forall tbl word vis sa sa' x gamma ,
-    Acc triple_lt (meas tbl (word, vis, sa))
-    -> ~ In x vis
-    -> pt_lookup x (peek word) tbl = Some gamma
-    -> Acc triple_lt (meas tbl (word, x :: vis, sa')).
-Proof.
-  intros.
-  eapply Acc_inv; eauto.
-  apply snd_lt; simpl.
-  apply NP.subset_cardinal_lt with (x := x).
-  - ND.fsetdec. 
-  - apply in_A_not_in_B_in_diff.
-    + apply in_list_iff_in_fromNtList.
-      eapply pt_lookup_in_nt_keys; eauto.
-    + apply not_in_list_iff_not_in_fromNtList; auto.
-  - ND.fsetdec.
-Defined.
-
-Lemma hole3 :
-  forall tbl word vis sa sa' tri' x gamma,
-  ~ In x vis
-  -> pt_lookup x (peek word) tbl = Some gamma
-  -> triple_le (meas tbl tri') (meas tbl (word, x :: vis, sa'))
-  -> triple_lt (meas tbl tri') (meas tbl (word, vis, sa)).
-Proof.
-  intros.
-  eapply triple_le_lt_trans; eauto.
-  apply snd_lt; simpl.
-  (* to do: factor out this part *)
-  apply NP.subset_cardinal_lt with (x := x).
-  - ND.fsetdec. 
-  - apply in_A_not_in_B_in_diff.
-    + apply in_list_iff_in_fromNtList.
-      eapply pt_lookup_in_nt_keys; eauto.
-    + apply not_in_list_iff_not_in_fromNtList; auto.
-  - ND.fsetdec.
-Defined.
-
-Lemma hole4 :
-  forall tbl word vis sa,
-    triple_le (meas tbl (word, vis, sa)) (meas tbl (word, vis, sa)).
-Proof.
-  intros.
-  right; auto.
-Defined.
-
-Lemma hole5 :
-  forall tbl word vis sa sym gamma,
-  Acc triple_lt (meas tbl (word, vis, sa))
-  -> sa = G_arg gamma
-  -> Acc triple_lt (meas tbl (word, vis, F_arg sym)).
-Proof.
-  intros; subst.
-  eapply Acc_inv; eauto.
-  apply thd_lt; red; auto.
-Defined.
-
-Lemma hole6 :
-  forall tbl word vis sa gamma sym gamma' tri' word' vis' sa',
-  Acc triple_lt (meas tbl (word, vis, sa))
-  -> sa = G_arg gamma
-  -> triple_lt (meas tbl tri') (meas tbl (word, vis, F_arg sym))
-  -> tri' = (word', vis', sa')
-  -> Acc triple_lt (meas tbl (word', vis', G_arg gamma')).
-Proof.
-  intros tbl word vis sa gamma sym gamma' tri' word' vis' sa' Ha Hsa Hlt Htri'; subst; simpl in *.
-  eapply Acc_inv; eauto.
-  inv Hlt.
-  - apply fst_lt; auto.
-  - assert (H : List.length word' = List.length word) by auto.
-    rewrite H.
-    apply snd_lt; auto.
-  - exfalso.
-    (* LEMMA *)
-    destruct sa'.
-    + simpl in *.
-      red in H0.
-      destruct H0.
-      congruence.
-    + simpl in *.
-      red in H0.
-      destruct H0.
-      congruence.
-Defined.
-
-Lemma hole7 :
-  forall tbl word word' vis vis' sa sa' tri' tri'' sym gamma,
-    triple_le (meas tbl tri'') (meas tbl (word', vis', G_arg gamma))
-    -> triple_lt (meas tbl tri') (meas tbl (word, vis, F_arg sym))
-    -> tri' = (word', vis', sa')
-    -> triple_le (meas tbl tri'') (meas tbl (word, vis, sa)).
-Proof.
-  intros; subst.
-  left.
-  destruct H.
-  - eapply triple_lt_trans; eauto.
-    inv H0.
-    + apply fst_lt; auto.
-    + assert (Hl : List.length word' = List.length word) by auto.
-      simpl.
-      rewrite Hl.
-      apply snd_lt; auto.
-    + exfalso.
-      destruct sa'.
-      * simpl in *; red in H2; destruct H2; congruence.
-      * simpl in *; red in H2; destruct H2; congruence.
-  - rewrite H.
-    (* LEMMA *)
-    inv H0.
-    + apply fst_lt; auto.
-    + assert (Hl : List.length word' = List.length word) by auto.
-      simpl.
-      rewrite Hl.
-      apply snd_lt; auto.
-    + exfalso.
-      destruct sa'.
-      * simpl in *; red in H2; destruct H2; congruence.
-      * simpl in *; red in H2; destruct H2; congruence.
-Defined.
-  
-Fixpoint parse5 (tbl     : parse_table)
-         (word : list string)
-         (vis : list nonterminal)
-         (sa : sym_arg)
-         (a       : Acc triple_lt (meas tbl (word, vis, sa)))
-         {struct a}
-  : sum parse_failure
-        (sum (list tree * {tri' | triple_le (meas tbl tri') (meas tbl (word, vis, sa))})
-             (tree      * {tri' | triple_lt (meas tbl tri') (meas tbl (word, vis, sa))})) :=
-  match sa as sa' return sa = sa' -> _ with
-          | F_arg sym =>
-            fun Hsa => match sym with
-                       | T y  => match word as w return word = w -> _ with
-                                 | [] => fun _ => inl (Mismatch "error message" word)
-                                 | token :: word' =>
-                                   if beqString y token then
-                                     fun Hword =>
-                                       inr (inr (Leaf y, exist _ (word', nil, sa) (hole1 _ _ _ _ _ _ _)))
-                                   else
-                                     fun _ => inl (Mismatch "error message" word)
-                                 end eq_refl
-                       | NT x =>
-                         match List.in_dec NT_as_DT.eq_dec x vis with
-                         | left _ => inl (LeftRec (x :: vis))
-                         | right Hnin =>
-                           match ptlk_dec x (peek word) tbl with
-                           | inl _ => inl (Mismatch "error message" word)
-                           | inr (exist _ gamma Hlk) =>
-                             (* Why do I need these two wildcards? *)
-                             match parse5 (*tbl word (x :: vis) (G_arg gamma) *) (hole2 (G_arg gamma) _ a Hnin Hlk) with 
-                                        | inl pf => inl pf
-                                        | inr (inr _) => inl Error
-                                        | inr (inl (sts, exist _ tri' Htri')) =>
-                                          inr (inr (Node x sts, exist _ tri' (hole3 _ _ Hnin Hlk Htri')))
-                                        end
-                           end
-                         end
-                       end
-          | G_arg gamma =>
-            fun Hsa => match gamma as g return gamma = g -> _ with
-                       | nil =>
-                         fun _ => inr (inl (nil, exist _ (word, vis, sa) (hole4 _ _ _ _)))
-                       | sym :: gamma' =>
-                         fun Hgamma => match parse5 (* tbl word vis (F_arg sym) *) (hole5 sym a Hsa) with (* tbl word vis F_arg sym (if_acc_gamma_then_acc_sym tbl a _ Hsa Hgamma) with *)
-                                       | inl pf => inl pf
-                                       | inr (inl _) => inl Error
-                                       | inr (inr (lSib, exist _ tri' Htri')) =>
-                                         match tri' as tri'2 return tri' = tri'2 -> _ with
-                                         | (word', vis', _) =>
-                                           fun Htri'eq => match parse5 (* tbl word' vis' (G_arg gamma') *) (hole6 gamma a Hsa Htri' Htri'eq) with (* tbl word' vis' (G_arg gamma') (acc_triple_lt_trans _ a _ Hsa Hgamma Htri') with*)
-                                                          | inl pf => inl pf
-                                                          | inr (inr _) => inl Error
-                                                          | inr (inl (rSibs, exist _ tri'' Htri'')) =>
-                                                            inr (inl (lSib :: rSibs, exist _ tri'' (hole7 _ _ Htri'' Htri' Htri'eq)))
-                                                          end
-                                         end eq_refl
-                                       end
-                       end eq_refl
-  end eq_refl.
-
-Lemma foo :
-  forall tbl word vis sa (a : Acc triple_lt (meas tbl (word, vis, sa))),
-    parse5 a =
-    match sa as sa' return sa = sa' -> _ with
-          | F_arg sym =>
-            fun Hsa => match sym with
-                       | T y  => match word as w return word = w -> _ with
-                                 | [] => fun _ => inl (Mismatch "error message" word)
-                                 | token :: word' =>
-                                   if beqString y token then
-                                     fun Hword =>
-                                       inr (inr (Leaf y, exist _ (word', nil, sa) (hole1 _ _ _ _ _ _ _)))
-                                   else
-                                     fun _ => inl (Mismatch "error message" word)
-                                 end eq_refl
-                       | NT x =>
-                         match List.in_dec NT_as_DT.eq_dec x vis with
-                         | left _ => inl (LeftRec (x :: vis))
-                         | right Hnin =>
-                           match ptlk_dec x (peek word) tbl with
-                           | inl _ => inl (Mismatch "error message" word)
-                           | inr (exist _ gamma Hlk) =>
-                             (* Why do I need these two wildcards? *)
-                             match parse5 (*tbl word (x :: vis) (G_arg gamma) *) (hole2 (G_arg gamma) _ a Hnin Hlk) with 
-                                        | inl pf => inl pf
-                                        | inr (inr _) => inl Error
-                                        | inr (inl (sts, exist _ tri' Htri')) =>
-                                          inr (inr (Node x sts, exist _ tri' (hole3 _ _ Hnin Hlk Htri')))
-                                        end
-                           end
-                         end
-                       end
-          | G_arg gamma =>
-            fun Hsa => match gamma as g return gamma = g -> _ with
-                       | nil =>
-                         fun _ => inr (inl (nil, exist _ (word, vis, sa) (hole4 _ _ _ _)))
-                       | sym :: gamma' =>
-                         fun Hgamma => match parse5 (* tbl word vis (F_arg sym) *) (hole5 sym a Hsa) with (* tbl word vis F_arg sym (if_acc_gamma_then_acc_sym tbl a _ Hsa Hgamma) with *)
-                                       | inl pf => inl pf
-                                       | inr (inl _) => inl Error
-                                       | inr (inr (lSib, exist _ tri' Htri')) =>
-                                         match tri' as tri'2 return tri' = tri'2 -> _ with
-                                         | (word', vis', _) =>
-                                           fun Htri'eq => match parse5 (* tbl word' vis' (G_arg gamma') *) (hole6 gamma a Hsa Htri' Htri'eq) with (* tbl word' vis' (G_arg gamma') (acc_triple_lt_trans _ a _ Hsa Hgamma Htri') with*)
-                                                          | inl pf => inl pf
-                                                          | inr (inr _) => inl Error
-                                                          | inr (inl (rSibs, exist _ tri'' Htri'')) =>
-                                                            inr (inl (lSib :: rSibs, exist _ tri'' (hole7 _ _ Htri'' Htri' Htri'eq)))
-                                                          end
-                                         end eq_refl
-                                       end
-                       end eq_refl
-    end eq_refl.
-Proof.
-  intros.
-  unfold parse5.
-  simpl.
-  destruct a. (* this is the key! *)
-  auto.
-Qed.
-      
-Lemma parse5_sym_ret_inr :
-  forall (tbl : parse_table)
-         (word : list string)
-         (vis : list nonterminal)
-         (sa : sym_arg)
-         e,
-    parse5 (triple_lt_wf (meas tbl (word, vis, sa))) = inr e
-    -> forall (sym : symbol),
-      sa = F_arg sym
-      -> isRight e = true.
-Proof.
-  intros; subst; simpl in *.
-  destruct sym.
-  - destruct word.
-    + congruence.
-    + destruct (beqString t s) eqn:Hbeq.
-      * inv H.
-        auto.
-      * congruence. 
-  - destruct (in_dec ND.F.eq_dec n vis).
-    + congruence.
-    + destruct (ptlk_dec n (peek word) tbl). 
-      * congruence.
-      * destruct s as [gamma Hlk].
-        repeat match goal with
-               | H : context[match ?X with
-                             | _ => _
-                             end] |- _ =>
-                 destruct X
-               end.
-        -- congruence.
-        -- inv H; auto.
-        -- congruence.
-Qed.
-
-Fixpoint parse6 (tbl     : parse_table)
-         (word : list string)
-         (vis : list nonterminal)
-         (sa : sym_arg)
-         (a       : Acc triple_lt (meas tbl (word, vis, sa)))
-         {struct a}
-  : sum parse_failure
-        (tree * {tri' | triple_lt (meas tbl tri') (meas tbl (word, vis, sa))}) :=
-  match sa as sa' return sa = sa' -> _ with
-  | G_arg _ => fun _ => inl Error
-  | F_arg sym =>
-    fun Hsa => match sym with
-               | T y => match word as w return word = w -> _ with
-                        | [] => fun _ => inl (Mismatch "error message" word)
-                        | token :: word' =>
-                          if beqString y token then
-                            fun Hword =>
-                              inr (Leaf y, exist _ (word', nil, sa) (hole1 _ _ _ _ _ _ _))
-                          else
-                            fun _ => inl (Mismatch "error message" word)
-                        end eq_refl
-               | NT x =>
-                 match List.in_dec NT_as_DT.eq_dec x vis with
-                 | left _ => inl (LeftRec (x :: vis))
-                 | right Hnin =>
-                   match ptlk_dec x (peek word) tbl with
-                   | inl _ => inl (Mismatch "error message" word)
-                   | inr (exist _ gamma Hlk) =>
-                     match parseForest6 (hole2 (G_arg gamma) _ a Hnin Hlk) with 
-                     | inl pf => inl pf
-                     | inr (sts, exist _ tri' Htri') =>
-                       inr (Node x sts, exist _ tri' (hole3 _ _ Hnin Hlk Htri'))
-                     end
-                   end
-                 end
-               end
-  end eq_refl
-with parseForest6 (tbl     : parse_table)
-                  (word : list string)
-                  (vis : list nonterminal)
-                  (sa : sym_arg)
-                  (a       : Acc triple_lt (meas tbl (word, vis, sa)))
-                  {struct a}
-     : sum parse_failure
-           (list tree * {tri' | triple_le (meas tbl tri') (meas tbl (word, vis, sa))}) :=
-       match sa as sa' return sa = sa' -> _ with
-       | F_arg _ => fun _ => inl Error
-       | G_arg gamma =>
-         fun Hsa => match gamma as g return gamma = g -> _ with
-                    | nil =>
-                      fun _ => inr (nil, exist _ (word, vis, sa) (hole4 _ _ _ _))
-                    | sym :: gamma' =>
-                      fun Hgamma => match parse6 (hole5 sym a Hsa) with
-                                    | inl pf => inl pf
-                                    | inr (lSib, exist _ tri' Htri') =>
-                                      match tri' as tri'2 return tri' = tri'2 -> _ with
-                                      | (word', vis', _) =>
-                                        fun Htri'eq => match parseForest6 (hole6 gamma a Hsa Htri' Htri'eq) with
-                                                       | inl pf => inl pf
-                                                       | inr (rSibs, exist _ tri'' Htri'') =>
-                                                         inr (lSib :: rSibs, exist _ tri'' (hole7 _ _ Htri'' Htri' Htri'eq))
-                                                       end
-                                      end eq_refl
-                                    end
-                    end eq_refl
-       end eq_refl.
-
-Lemma parse_t_ret_leaf :
-  forall tbl word vis sa y (a : Acc triple_lt (meas tbl (word, vis, sa))) tr tri' pf,
-    sa = F_arg (T y)
-    -> parse6 a = inr (tr, exist _ tri' pf)
-    -> isLeaf tr = true.
-Proof.
-  intros.
-  unfold parse6 in H; destruct a; subst; simpl in *.
-  - destruct word.
-    + congruence.
-    + destruct (beqString y s).
-      * inv H0.
-        auto.
-      * congruence.
-Qed.
-
-Ltac crush :=
-  repeat (simpl in *;
-          match goal with
-          | H : context[match ?X with | _ => _ end] |- _ =>
-            let Heq := fresh "Heq" in
-            destruct X eqn:Heq
-          | H : inr _ = inr _ |- _ => inv H
-
-          | H : inl _ = inr _ |- _ => congruence
-          | H : isNode (Leaf _) = true |- _ => inv H
-          end;
-          auto).
-          
-Lemma parse_nt_ret_node :
-  forall tbl word vis x (a : Acc triple_lt (meas tbl (word, vis, F_arg (NT x)))) tr tri' pf,
-    parse6 a = inr (tr, exist _ tri' pf)
-    -> isNode tr = true.
-Proof.
-  intros.
-  destruct a.
-  crush.
-Qed.
-
-(*
-Require Import Lib.Lemmas.
-Require Import LL1.Derivation.
-
-Lemma parse_correct' :
-  forall (g   : grammar)
-         (tbl : parse_table),
-    parse_table_for tbl g
-    -> forall (input rem : list string)
-              (vis vis' : list nonterminal)
-              (sym   : symbol)
-              (sa' : sym_arg)
-              (a : Acc triple_lt (meas tbl (input, vis, F_arg sym)))
-              (tr : tree)
-              pf,
-      parse6 a = inr (tr, exist _ (rem, vis', sa') pf)
-      -> exists word,
-        word ++ rem = input
-        /\ (@sym_derives_prefix g) sym word tr rem.
-Proof.
-  intros.
-  induction tr as [ s
-                  | s f IHpf
-                  |
-                  | tr IHp f IHpf ]
-                    using tree_nested_ind with
-      
-      (P := fun tr =>
-              parse6 a = inr (tr, exist _ (rem, vis', sa') pf)
-              -> exists word : list string,
-                word ++ rem = input /\ sym_derives_prefix sym word tr rem)
-      
-      (Q := fun f =>
-              forall input rem vis vis' gamma sa' pf (a : Acc triple_lt (meas tbl (input, vis, G_arg gamma))),
-                parseForest6 a = inr (f, exist _ (rem, vis', sa') pf)
-                -> exists word,
-                  word ++ rem = input
-                  /\ gamma_derives_prefix gamma word f rem).
-
-  - destruct a.
-    destruct sym as [y | x] eqn:Hsym.
-    + destruct input as [| token word'].
-      * crush.
-      * crush.
-        exists [token]; split; auto.
-        apply beqString_eq in Heq; subst.
-        constructor.
-    + crush.
-
-  - destruct a.
-    destruct sym as [y | x].
-    + crush.
-    + simpl in H0.
-      destruct (in_dec ND.F.eq_dec x vis).
-      * crush.
-      * destruct (ptlk_dec x (peek input) tbl).
-        -- crush.
-        -- destruct s0 as [gamma Hlk].
-           crush.
-Abort.
- *)
-
-Fixpoint pf7 (p : parse_table -> symbol -> list string -> list nonterminal -> (option tree * list string))
-             (tbl : parse_table) 
-             (gamma : list symbol)
-             (input : list string)
-             (vis : list nonterminal)
-             : (option (list tree) * list string) :=
-  match gamma with
-  | nil => (Some nil, input)
-  | sym :: gamma' =>
-    match p tbl sym input vis with
-    | (None, _) => (None, input)
-    | (Some lSib, input') =>
-      match pf7 p tbl gamma' input' [] with
-      | (None, _) => (None, input)
-      | (Some rSibs, input'') =>
-        (Some (lSib :: rSibs), input'')
-      end
-    end
-  end.
-
-Definition m7 (tbl : parse_table)
-              (vis : list nonterminal) :=
-  NtSet.cardinal (NtSet.diff (fromNtList (nt_keys tbl))
-                             (fromNtList vis)).
-
-Program Fixpoint p7 (tbl : parse_table)
-                    (sym : symbol)
-                    (input : list string)
-                    (vis : list nonterminal)
-                    {measure (m7 tbl vis)}
-  : (option tree * list string) :=
-  match (sym, input) with
-  | (T _, nil) => (None, input)
-  | (T y, token :: input') =>
-    if beqString y token then
-      (Some (Leaf y), input')
-    else
-      (None, input)
-  | (NT x, _) =>
-    match pt_lookup x (peek input) tbl with
-    | None => (None, input)
-    | Some gamma =>
-      if List.in_dec NT_as_DT.eq_dec x vis then
-        (None, input)
-      else
-        let fix pf7 gamma input :=
-            match gamma with
-            | nil => (Some nil, input)
-            | sym :: gamma' =>
-              match p7 tbl sym input (x :: vis) with
-              | (None, _) => (None, input)
-              | (Some lSib, input') =>
-                match pf7 gamma' input' with
-                | (None, _) => (None, input)
-                | (Some rSibs, input'') =>
-                  (Some (lSib :: rSibs), input'')
-                end
-              end
-            end
-        in  match pf7 gamma input with
-            | (None, _) => (None, input)
-            | (Some sts, input') =>
-              (Some (Node x sts), input')
-            end
-    end
-  end.
-Next Obligation.
-  unfold m7; simpl.
-  apply NP.subset_cardinal_lt with (x := x).
-  - ND.fsetdec.
-  - apply in_A_not_in_B_in_diff.
-    + apply in_list_iff_in_fromNtList.
-      eapply pt_lookup_in_nt_keys; eauto.
-    + apply not_in_list_iff_not_in_fromNtList; auto.
-  - ND.fsetdec.
-Defined.
-
-Lemma p8_hole :
-  forall tbl vis x input gamma,
-  Acc lt (m7 tbl vis)
-  -> pt_lookup x (peek input) tbl = Some gamma
-  -> ~ In x vis
-  -> Acc lt (m7 tbl (x :: vis)).
-Proof.
-  intros.
-  eapply Acc_inv; eauto.
-  unfold m7; simpl.
-  apply NP.subset_cardinal_lt with (x := x).
-  - ND.fsetdec.
-  - apply in_A_not_in_B_in_diff.
-    + apply in_list_iff_in_fromNtList.
-      eapply pt_lookup_in_nt_keys; eauto.
-    + apply not_in_list_iff_not_in_fromNtList; auto.
-  - ND.fsetdec.
-Defined.
-
-Fixpoint p8 (tbl : parse_table)
-         (sym : symbol)
-         (input : list string)
-         (vis : list nonterminal)
-         (a : Acc lt (m7 tbl vis))
-         {struct a}
-  : (option tree * list string) :=
-  match (sym, input) with
-  | (T _, nil) => (None, input)
-  | (T y, token :: input') =>
-    if beqString y token then
-      (Some (Leaf y), input')
-    else
-      (None, input)
-  | (NT x, _) =>
-    match ptlk_dec x (peek input) tbl with
-    | inl _ => (None, input)
-    | inr (exist _ gamma Hlk) =>
-      match List.in_dec NT_as_DT.eq_dec x vis with
-      | left _ => (None, input)
-      | right Hnin => 
-        let fix pf8 gamma input :=
-            match gamma with
-            | nil => (Some nil, input)
-            | sym :: gamma' =>
-              match p8 tbl sym input (x :: vis) (p8_hole _ _ _ _ a Hlk Hnin) with
-              | (None, _) => (None, input)
-              | (Some lSib, input') =>
-                match pf8 gamma' input' with
-                | (None, _) => (None, input)
-                | (Some rSibs, input'') =>
-                  (Some (lSib :: rSibs), input'')
-                end
-              end
-            end
-        in  match pf8 gamma input with
-            | (None, _) => (None, input)
-            | (Some sts, input') =>
-              (Some (Node x sts), input')
-            end
-      end
-    end
-  end.
-
-Lemma p8_eq_body :
-  forall tbl sym input vis a,
-    p8 tbl sym input vis a =
-    match (sym, input) with
-    | (T _, nil) => (None, input)
-    | (T y, token :: input') =>
-      if beqString y token then
-        (Some (Leaf y), input')
-      else
-        (None, input)
-    | (NT x, _) =>
-      match ptlk_dec x (peek input) tbl with
-      | inl _ => (None, input)
-      | inr (exist _ gamma Hlk) =>
-        match List.in_dec NT_as_DT.eq_dec x vis with
-        | left _ => (None, input)
-        | right Hnin => 
-          let fix pf8 gamma input :=
-              match gamma with
-              | nil => (Some nil, input)
-              | sym :: gamma' =>
-                match p8 tbl sym input (x :: vis) (p8_hole _ _ _ _ a Hlk Hnin) with
-                | (None, _) => (None, input)
-                | (Some lSib, input') =>
-                  match pf8 gamma' input' with
-                  | (None, _) => (None, input)
-                  | (Some rSibs, input'') =>
-                    (Some (lSib :: rSibs), input'')
-                  end
-                end
-              end
-          in  match pf8 gamma input with
-              | (None, _) => (None, input)
-              | (Some sts, input') =>
-                (Some (Node x sts), input')
-              end
-        end
-      end
-    end.
-Proof.
-  intros.
-  unfold p8.
-  destruct a.
-  destruct sym.
-  - destruct input; auto.
-  - destruct (ptlk_dec n (peek input) tbl); auto.
-Qed.
-
-Ltac dest_match :=
-  repeat match goal with
-         | H : context[match ?x with | _ => _ end] |- _ =>
-           destruct x
-         end.
-
-Lemma p8_t_ret_leaf :
-  forall tbl y word vis a tr rem,
-    p8 tbl (T y) word vis a = (Some tr, rem)
-    -> isLeaf tr = true.
-Proof.
-  intros.
-  destruct a.
-  rewrite p8_eq_body in H.
-  dest_match; try inv H; auto.
-Qed.
-
-Lemma p8_nt_ret_node :
-  forall tbl x word vis a tr rem,
-    p8 tbl (NT x) word vis a = (Some tr, rem)
-    -> isNode tr = true.
-Proof.
-  intros.
-  rewrite p8_eq_body in H.
-  dest_match; try inv H.
-  destruct x0; simpl in *.
-  - inv H1; auto.
-  - dest_match; try congruence.
-    subst.
-    inv H1; auto.
-Qed.
-
-Require Import LL1.Derivation.  
-
-Lemma p8_sound' :
-  forall (g   : grammar)
-         (tbl : parse_table),
-    parse_table_for tbl g
-    -> forall (tr        : tree)
-              (sym       : symbol)
-              (input rem : list terminal)
-              (vis : list nonterminal)
-              a,
-      p8 tbl sym input vis a = (Some tr, rem)
-      -> exists word,
-        word ++ rem = input
-        /\ (@sym_derives_prefix g) sym word tr rem.
-Proof.
-  intros g tbl Htbl tr. 
-  induction tr as [ s
-                  | s f IHpf
-                  |
-                  | tr IHp f IHpf ]
-                    using tree_nested_ind with
-      
-      (P := fun tr =>
-              forall (sym : symbol) (input rem : list terminal)
-                     (vis : list nonterminal) (a : Acc lt (m7 tbl vis)),
-                p8 tbl sym input vis a = (Some tr, rem) ->
-                exists word : list terminal,
-                  word ++ rem = input /\
-                  sym_derives_prefix sym word tr rem)
-
-      (Q := fun f =>
-              forall gamma input rem vis a,
-                (fix pf8 gamma input :=
-                   match gamma with
-                   | nil => (Some nil, input)
-                   | sym :: gamma' =>
-                     match p8 tbl sym input vis a with
-                     | (None, _) => (None, input)
-                     | (Some lSib, input') =>
-                       match pf8 gamma' input' with
-                       | (None, _) => (None, input)
-                       | (Some rSibs, input'') =>
-                         (Some (lSib :: rSibs), input'')
-                       end
-                     end
-                   end) gamma input = (Some f, rem)
-                -> exists word,
-                  word ++ rem = input
-                  /\ gamma_derives_prefix gamma word f rem).
-
-  - intros.
-    destruct sym as [y|x].
-    + rewrite p8_eq_body in H.
-      destruct input; try congruence.
-      destruct (beqString y t) eqn:Hb; try congruence.
-      inv H.
-      apply beqSym_eq in Hb; subst.
-      eexists; split.
-      * replace (t :: rem) with ([t] ++ rem); auto.
-      * constructor.
-    + apply p8_nt_ret_node in H.
-      inv H.
-
-  - intros.
-    destruct sym as [y|x].
-    + apply p8_t_ret_leaf in H; inv H.
-    + rewrite p8_eq_body in H.
-      destruct (ptlk_dec x (peek input) tbl); try congruence.
-      destruct s0 as [gamma Hlk].
-      destruct (in_dec ND.F.eq_dec x vis); try congruence.
-      progress simpl in H.
-      match goal with
-      | H : context[?f gamma input] |- _ =>
-        destruct (f gamma input) eqn:Hpf
-      end.
-      destruct o; try congruence.
-      inv H.
-      specialize (IHpf gamma input rem (s :: vis) (p8_hole tbl vis s input a Hlk n)).
-      apply IHpf in Hpf; clear IHpf.
-      destruct Hpf as [word [Happ Hd]].
-      subst.
-      eexists; split; eauto.
-      apply Htbl in Hlk.
-      destruct Hlk.
-      econstructor; eauto.
-
-  - intros.
-    destruct gamma.
-    + inv H.
-      exists nil; split; auto.
-      constructor.
-    + destruct (p8 tbl s input vis a).
-      * destruct o; try congruence.
-        match goal with
-        | H : context[?f ?a ?b] |- _ =>
-          destruct (f a b)
-        end.
-        destruct o; try congruence.
-        
-  - intros.
-    destruct gamma; try congruence.
-    destruct (p8 tbl s input vis a) eqn:Hp.
-    destruct o; try congruence.
-    match goal with
-    | H : context[?f ?a ?b] |- _ =>
-      destruct (f a b) eqn:Hpf
-    end.
-    destruct o; try congruence.
-    inv H.
-    apply IHp in Hp; clear IHp.
-    apply IHpf with (a := a) in Hpf.
-    destruct Hp as [wpre [Happ Hs]].
-    destruct Hpf as [wsuf [Happ' Hg]].
-    subst.
-    exists (wpre ++ wsuf).
-    split.
-    + rewrite app_assoc; auto.
-    + constructor; auto.
-Qed.
 
 Definition X := 0.
 Definition Y := 1.
@@ -1637,10 +224,6 @@ Definition yy_grammar :=
 
 Require Import EndToEnd.
 
-Eval compute in match parseTableOf yy_grammar with
-                | None => None
-                | Some tbl => Some (p8 tbl (NT X) ["a"] [] (lt_wf (m7 tbl [])))
-                end.
 
 Definition a_generator :=
   {|
@@ -1649,140 +232,11 @@ Definition a_generator :=
                      (X, [])]
   |}.
 
-Eval compute in parseTableOf a_generator.
-
-(* This example shows that p8 is incomplete as written --
-   a valid LL(1) parser generated with this grammar should
-   accept any sequence of a's *)
-Eval compute in match parseTableOf a_generator with
-                | None => None
-                | Some tbl => Some (p8 tbl
-                                       (NT X)
-                                       ["a"; "a"; "a"]
-                                       []
-                                       (lt_wf (m7 tbl [])))
-                end.
-
-Eval compute in match parseTableOf a_generator with
-                | None => None
-                | Some tbl => Some (parse tbl
-                                       (NT X)
-                                       ["a"; "a"; "a"]
-                                       17)
-                end.
-
 Definition lr_table :=
   ParseTable.add (X, LA "a") [NT Y; NT Z]
                  (ParseTable.add (Y, LA "a") []
                                  (ParseTable.add (Z, LA "a") [NT X]
                                                  (ParseTable.empty (list symbol)))).
-
-Eval compute in (p8 lr_table (NT X) ["a"] [] (lt_wf (m7 lr_table []))).
-
-Definition pair_lt := pair_lex nat nat lt lt.
-
-Definition m9 tbl (input : list string) vis :=
-  (List.length input, NtSet.cardinal
-                        (NtSet.diff (fromNtList (nt_keys tbl))                                     (fromNtList vis))).
-
-(* things to try today:
-
-   nested recursion--inner func is structurally recursive on gamma
-   + extra "lt fact" arg
-   + extra Acc arg
-
-   mutual recursion on Acc arg
-   + need "sym_arg order" relation in which gamma < x :: gamma
- *)
-
-Require Import Omega.
-Program Fixpoint p9 (tbl : parse_table)
-                    (sym : symbol)
-                    (input : list string)
-                    (vis : list nonterminal)
-                    {measure (m9 tbl input vis) (pair_lt)}
-  : (option tree * list string) :=
-  match (sym, input) with
-  | (T _, nil) => (None, input)
-  | (T y, token :: input') =>
-    if beqString y token then
-      (Some (Leaf y), input')
-    else
-      (None, input)
-  | (NT x, _) =>
-    match pt_lookup x (peek input) tbl with
-    | None => (None, input)
-    | Some gamma =>
-      if List.in_dec NT_as_DT.eq_dec x vis then
-        (None, input)
-      else
-        let fix pf9 gamma pf_input pf_vis (H : pair_lt (m9 tbl pf_input pf_vis) (m9 tbl input vis)) :=
-            match gamma with
-            | nil => (Some nil, pf_input)
-            | sym :: gamma' =>
-              match p9 tbl sym pf_input pf_vis with
-              | (None, _) => (None, input)
-              | (Some lSib, lrem) =>
-                match Compare_dec.lt_dec (List.length lrem) (List.length pf_input) with
-                | left Hlt =>
-                  match pf9 gamma' lrem [] _ with
-                  | (None, _) => (None, lrem)
-                  | (Some rSibs, rrem) =>
-                    (Some (lSib :: rSibs), rrem)
-                  end
-                | right Hnlt =>
-                  match pf9 gamma' pf_input pf_vis _ with
-                  | (None, _) => (None, pf_input)
-                  | (Some rSibs, rrem) =>
-                    (Some (lSib :: rSibs), rrem)
-                  end
-                end
-              end
-            end
-        in  match pf9 gamma input (x :: vis) _ with
-            | (None, _) => (None, input)
-            | (Some sts, input') =>
-              (Some (Node x sts), input')
-            end
-    end
-  end.
-Next Obligation.
-  apply pr_fst_lt.
-  clear Heq_anonymous2.
-  inv H.
-  - omega.
-  - omega.
-Defined.
-Next Obligation.
-  unfold m9; simpl in *.
-  apply pr_snd_lt.
-  apply NP.subset_cardinal_lt with (x := x).
-  - ND.fsetdec.
-  - apply in_A_not_in_B_in_diff.
-    + apply in_list_iff_in_fromNtList.
-      eapply pt_lookup_in_nt_keys; eauto.
-    + apply not_in_list_iff_not_in_fromNtList; auto.
-  - ND.fsetdec.
-Defined.
-Next Obligation.
-  apply measure_wf.
-  apply pair_lex_wf; apply lt_wf.
-Defined.
-
-Eval compute in match parseTableOf yy_grammar with
-                | None => None
-                | Some tbl => Some (p9 tbl (NT X) ["a"] [])
-                end.
-
-Eval compute in match parseTableOf a_generator with
-                | None => None
-                | Some tbl => Some (p9 tbl
-                                       (NT X)
-                                       ["a"; "a"; "a"]
-                                       [])
-                end.
-
-Eval compute in (p9 lr_table (NT X) ["a"] []).
 
 Inductive sa_order : sym_arg -> sym_arg -> Prop := 
 | f_lt_g : forall sym gamma,
@@ -1791,163 +245,57 @@ Inductive sa_order : sym_arg -> sym_arg -> Prop :=
     List.length gamma' < List.length gamma
     -> sa_order (G_arg gamma') (G_arg gamma).
 
-Definition m10 tbl (word : list string) (vis : list nonterminal) (sa : sym_arg) :=
+Definition meas tbl (word : list string) (vis : list nonterminal) (sa : sym_arg) :=
   (List.length word,
    NtSet.cardinal (NtSet.diff (fromNtList (nt_keys tbl))                                     (fromNtList vis)),
    sa).
 
-Definition lt10 : relation (nat * nat * sym_arg) :=
+Definition triple_lt : relation (nat * nat * sym_arg) :=
   triple_lex nat nat sym_arg lt lt sa_order.
 
-
-(* working towards mutual recursion *)
-Fixpoint p10 (tbl : parse_table)
-             (sym : symbol)
-             (input : list string)
-             (vis : list nonterminal)
-             (a : Acc lt10 (m10 tbl input vis (F_arg sym)))
-             {struct a}
-  : (option tree * list string).
-  refine (match (sym, input) with
-          | (T _, nil) => (None, input)
-          | (T y, token :: input') =>
-            if beqString y token then
-              (Some (Leaf y), input')
-            else
-              (None, input)
-          | (NT x, _) =>
-            match ptlk_dec x (peek input) tbl with
-            | inl _ => (None, input)
-            | inr (exist _ gamma Hlk) =>
-              match List.in_dec NT_as_DT.eq_dec x vis with
-              | left _ => (None, input)
-              | right Hnin => 
-                let fix pf10 (tbl : parse_table)
-                        (gamma : list symbol)
-                        (input : list string)
-                        (vis : list nonterminal)
-                        (a : Acc lt10 (m10 tbl input vis (G_arg gamma)))
-                        {struct a}
-                    : (option (list tree) * list string) :=
-                    match gamma as g return gamma = g -> _  with
-                    | nil => fun _ => (Some nil, input)
-                    | sym :: gamma' => fun Hg => 
-                                         match p10 tbl sym input vis _ with
-                                         | (None, _) => (None, input)
-                                         | (Some lSib, input') =>
-                                           match Compare_dec.lt_dec (List.length input') (List.length input) with
-                                           | left Hlt =>
-                                             match pf10 tbl gamma' input' [] _ with
-                                             | (None, _) => (None, input)
-                                             | (Some rSibs, input'') =>
-                                               (Some (lSib :: rSibs), input'')
-                                             end
-                                           | right Hnlt =>
-                                             match pf10 tbl gamma' input vis _ with
-                                             | (None, _) => (None, input)
-                                             | (Some rSibs, input'') =>
-                                               (Some (lSib :: rSibs), input'')
-                                             end
-                                           end
-                                         end
-                    end eq_refl
-              in  match pf10 tbl gamma input (x :: vis) _ with
-                  | (None, _) => (None, input)
-                  | (Some sts, input') =>
-                    (Some (Node x sts), input')
-                  end
-              end
-            end
-          end).
-  clear pf10.
-  eapply Acc_inv; eauto.
-  unfold m10; simpl.
-  apply snd_lt.
-  apply NP.subset_cardinal_lt with (x := x).
-  - ND.fsetdec.
-  - apply in_A_not_in_B_in_diff.
-    + apply in_list_iff_in_fromNtList.
-      eapply pt_lookup_in_nt_keys; eauto.
-    + apply not_in_list_iff_not_in_fromNtList; auto.
-  - ND.fsetdec.
-    Unshelve.
-    + eapply Acc_inv; eauto.
-      * unfold m10.
-        apply thd_lt.
-        constructor.
-    + eapply Acc_inv; eauto.
-      apply fst_lt; auto.
-    + eapply Acc_inv; eauto.
-      apply thd_lt.
-      constructor.
-      subst.
-      auto.
+Lemma sa_order_wf'' :
+  forall sym, Acc sa_order (F_arg sym).
+Proof.
+  intros.
+  constructor; intros a H.
+  inv H.
 Defined.
 
+Lemma sa_order_wf' :
+  forall n gamma,
+    List.length gamma < n
+    -> Acc sa_order (G_arg gamma).
+Proof.
+  induction n; intros gamma H; simpl in *.
+  - inv H.
+  - constructor; intros a Ha.
+    inv Ha; simpl in *.
+    + apply sa_order_wf''.
+    + apply IHn; omega.
+Defined.
 
 Theorem sa_order_wf : well_founded sa_order.
 Proof.
-  unfold well_founded.
-  intros a.
-  induction a.
-  - constructor; intros.
-    inv H.
-  - induction l.
-    + constructor; intros.
-      inv H.
-      * constructor; intros.
-        inv H.
-      * inv H2.
-    + constructor; intros.
-      inv H.
-      * constructor; intros.
-        inv H.
-      * destruct gamma'.
-        -- constructor; intros.
-           inv H.
-           ++ constructor; intros.
-              inv H.
-           ++ inv H3.
-        -- simpl in *.
-           constructor; intros.
-           inv H.
-           ++ constructor; intros.
-              inv H.
-           ++ simpl in *.
-              eapply Acc_inv; eauto.
-              constructor.
-              omega.
+  red; intros a; destruct a.
+  - apply sa_order_wf''.
+  - eapply sa_order_wf'; eauto.
 Defined.
 
-Extraction p10.
-
-Theorem lt10_wf : well_founded lt10.
+Theorem triple_lt_wf : well_founded triple_lt.
   apply triple_lex_wf; try apply lt_wf.
   apply sa_order_wf.
 Defined.
 
-Eval compute in match parseTableOf yy_grammar with
-                | None => None
-                | Some tbl => Some (p10 (lt10_wf (m10 tbl ["a"] [] (F_arg (NT X)))))
-                end.
-
-Eval compute in match parseTableOf a_generator with
-                | None => None
-                | Some tbl => Some (p10 (lt10_wf (m10 tbl ["a"; "a"; "a"] [] (F_arg (NT X)))))
-                end.
-
-Eval compute in (p10 (lt10_wf (m10 lr_table ["a"] [] (F_arg (NT X))))).
-
-Lemma p11_hole1 :
+Lemma hole1 :
   forall tbl input vis sa sa' x gamma,
-    Acc lt10 (m10 tbl input vis sa)
+    Acc triple_lt (meas tbl input vis sa)
     -> pt_lookup x (peek input) tbl = Some gamma
     -> ~ In x vis
-    -> Acc lt10 (m10 tbl input (x :: vis) sa').
+    -> Acc triple_lt (meas tbl input (x :: vis) sa').
 Proof.
   intros.
   eapply Acc_inv; eauto.
-  unfold m10.
+  unfold meas.
   apply snd_lt; simpl.
   apply NP.subset_cardinal_lt with (x := x); try ND.fsetdec.
   apply in_A_not_in_B_in_diff.
@@ -1956,32 +304,32 @@ Proof.
   - apply not_in_list_iff_not_in_fromNtList; auto.
 Defined.
 
-Lemma p11_hole2 :
+Lemma hole2 :
   forall tbl input vis gamma sym,
-    Acc lt10 (m10 tbl input vis (G_arg gamma))
-    -> Acc lt10 (m10 tbl input vis (F_arg sym)).
+    Acc triple_lt (meas tbl input vis (G_arg gamma))
+    -> Acc triple_lt (meas tbl input vis (F_arg sym)).
 Proof.
   intros.
   eapply Acc_inv; eauto.
   apply thd_lt; constructor.
 Defined.
 
-Lemma p11_hole3 :
+Lemma hole3 :
   forall tbl input input' vis vis' sa sa',
-    Acc lt10 (m10 tbl input vis sa)
+    Acc triple_lt (meas tbl input vis sa)
     -> List.length input' < List.length input
-    -> Acc lt10 (m10 tbl input' vis' sa').
+    -> Acc triple_lt (meas tbl input' vis' sa').
 Proof.
   intros.
   eapply Acc_inv; eauto.
   apply fst_lt; auto.
 Defined.
 
-Lemma p11_hole4 :
+Lemma hole4 :
   forall tbl input vis gamma sym gamma',
-    Acc lt10 (m10 tbl input vis (G_arg gamma))
+    Acc triple_lt (meas tbl input vis (G_arg gamma))
     -> gamma = sym :: gamma'
-    -> Acc lt10 (m10 tbl input vis (G_arg gamma')).
+    -> Acc triple_lt (meas tbl input vis (G_arg gamma')).
 Proof.
   intros.
   eapply Acc_inv; eauto.
@@ -1989,73 +337,13 @@ Proof.
   constructor; auto.
 Defined.
 
-Fixpoint p11 (tbl : parse_table)
-             (sym : symbol)
-             (input : list string)
-             (vis : list nonterminal)
-             (a : Acc lt10 (m10 tbl input vis (F_arg sym)))
-             {struct a}
-  : (option tree * list string).
-  refine (match (sym, input) with
-          | (T _, nil) => (None, input)
-          | (T y, token :: input') =>
-            if beqString y token then
-              (Some (Leaf y), input')
-            else
-              (None, input)
-          | (NT x, _) =>
-            match ptlk_dec x (peek input) tbl with
-            | inl _ => (None, input)
-            | inr (exist _ gamma Hlk) =>
-              match List.in_dec NT_as_DT.eq_dec x vis with
-              | left _ => (None, input)
-              | right Hnin => 
-                let fix pf11 (tbl : parse_table)
-                        (gamma : list symbol)
-                        (input : list string)
-                        (vis : list nonterminal)
-                        (a : Acc lt10 (m10 tbl input vis (G_arg gamma)))
-                        {struct a}
-                    : (option (list tree) * list string) :=
-                    match gamma as g return gamma = g -> _  with
-                    | nil => fun _ => (Some nil, input)
-                    | sym :: gamma' => fun Hg => 
-                                         match p11 tbl sym input vis (p11_hole2 _ a) with
-                                         | (None, _) => (None, input)
-                                         | (Some lSib, input') =>
-                                           match Compare_dec.lt_dec (List.length input') (List.length input) with
-                                           | left Hlt =>
-                                             match pf11 tbl gamma' input' [] (p11_hole3 _ _ _ a Hlt) with
-                                             | (None, _) => (None, input)
-                                             | (Some rSibs, input'') =>
-                                               (Some (lSib :: rSibs), input'')
-                                             end
-                                           | right Hnlt =>
-                                             match pf11 tbl gamma' input vis (p11_hole4 a Hg) with
-                                             | (None, _) => (None, input)
-                                             | (Some rSibs, input'') =>
-                                               (Some (lSib :: rSibs), input'')
-                                             end
-                                           end
-                                         end
-                    end eq_refl
-              in  match pf11 tbl gamma input (x :: vis) (p11_hole1 _ _ a Hlk Hnin) with
-                  | (None, _) => (None, input)
-                  | (Some sts, input') =>
-                    (Some (Node x sts), input')
-                  end
-              end
-            end
-          end).
-Defined.
-
-Fixpoint p12 (tbl : parse_table)
-             (sym : symbol)
-             (input : list string)
-             (vis : list nonterminal)
-             (a : Acc lt10 (m10 tbl input vis (F_arg sym)))
-             {struct a}
-             : (option tree * list string) := 
+Fixpoint p (tbl : parse_table)
+         (sym : symbol)
+         (input : list string)
+         (vis : list nonterminal)
+         (a : Acc triple_lt (meas tbl input vis (F_arg sym)))
+         {struct a}
+         : (option tree * list string) := 
   match (sym, input) with
   | (T _, nil) => (None, input)
   | (T y, token :: input') =>
@@ -2064,42 +352,42 @@ Fixpoint p12 (tbl : parse_table)
     else
       (None, input)
   | (NT x, _) =>
-    match pt_lookup x (peek input) tbl as o return pt_lookup x (peek input) tbl = o -> _ with
-    | None => fun _ => (None, input)
-    | Some gamma =>
-      fun Hlk => match List.in_dec NT_as_DT.eq_dec x vis with
-                 | left _ => (None, input)
-                 | right Hnin => 
-                   match pf12 (p11_hole1 (G_arg gamma) x a Hlk Hnin) with
-                   | (None, _) => (None, input)
-                   | (Some sts, input') =>
-                     (Some (Node x sts), input')
-                   end
-                 end
-    end eq_refl
+    match ptlk_dec x (peek input) tbl with
+    | inl _ => (None, input)
+    | inr (exist _ gamma Hlk) =>
+      match List.in_dec NT_as_DT.eq_dec x vis with
+      | left _ => (None, input)
+      | right Hnin => 
+        match pf tbl gamma input (x :: vis) (hole1 _ _ _ _  _ _ _ a Hlk Hnin) with
+        | (None, _) => (None, input)
+        | (Some sts, input') =>
+          (Some (Node x sts), input')
+        end
+      end
+    end
   end
-with pf12 (tbl : parse_table)
-          (gamma : list symbol)
-          (input : list string)
-          (vis : list nonterminal)
-          (a : Acc lt10 (m10 tbl input vis (G_arg gamma)))
-          {struct a}
-     : (option (list tree) * list string) :=
+with pf (tbl : parse_table)
+        (gamma : list symbol)
+        (input : list string)
+        (vis : list nonterminal)
+        (a : Acc triple_lt (meas tbl input vis (G_arg gamma)))
+        {struct a}
+        : (option (list tree) * list string) :=
        match gamma as g return gamma = g -> _  with
        | nil => fun _ => (Some nil, input)
        | sym :: gamma' => fun Hg => 
-                            match p12 (p11_hole2 sym a) with
+                            match p tbl sym input vis (hole2 _ _ _ _ _ a) with
                             | (None, _) => (None, input)
                             | (Some lSib, input') =>
                               match Compare_dec.lt_dec (List.length input') (List.length input) with
                               | left Hlt =>
-                                match pf12 (p11_hole3 input' [] (G_arg gamma') a Hlt) with
+                                match pf tbl gamma' input' [] (hole3 _ _ _ _ _ _ _ a Hlt) with
                                 | (None, _) => (None, input)
                                 | (Some rSibs, input'') =>
                                   (Some (lSib :: rSibs), input'')
                                 end
                               | right Hnlt =>
-                                match pf12 (p11_hole4 a Hg) with
+                                match pf tbl gamma' input vis (hole4 _ _ _ _ _ _ a Hg) with
                                 | (None, _) => (None, input)
                                 | (Some rSibs, input'') =>
                                   (Some (lSib :: rSibs), input'')
@@ -2108,25 +396,329 @@ with pf12 (tbl : parse_table)
                             end
        end eq_refl.
 
-Extraction p12.
+Definition parse_wrapper tbl sym input vis :=
+  p tbl sym input vis (triple_lt_wf (meas tbl input vis (F_arg sym))).
 
 Eval compute in match parseTableOf yy_grammar with
                 | None => None
-                | Some tbl => Some (p12 (lt10_wf (m10 tbl ["a"] [] (F_arg (NT X)))))
+                | Some tbl => Some (parse_wrapper tbl (NT X) ["a"] [])
                 end.
 
 Eval compute in match parseTableOf a_generator with
                 | None => None
-                | Some tbl => Some (p12 (lt10_wf (m10 tbl ["a"; "a"; "a"] [] (F_arg (NT X)))))
+                | Some tbl => Some (parse_wrapper tbl (NT X) ["a"; "a"; "a"] [])
                 end.
 
-Eval compute in (p10 (lt10_wf (m10 lr_table ["a"] [] (F_arg (NT X))))).
+Eval compute in parse_wrapper lr_table (NT X) ["a"] [].
+
+Ltac step_h := match goal with
+               | H : context[match ?x with | _ => _ end] |- _ => destruct x
+              end.
+
+Ltac step_h_eq s := let Heq := fresh s in
+                    match goal with
+                    | H : context[match ?x with | _ => _ end] |- _ =>
+                      destruct x eqn:Heq
+                    end.
+
+Ltac step_g := match goal with
+               | |- context[match ?x with | _ => _ end] => destruct x
+               end.
+
+Ltac step := simpl in *; (first [step_h | step_g]); auto.
+Ltac step_eq s := simpl in *; (first [step_h_eq s | step_g]); auto.
+Ltac cr := repeat step.
+Ltac cr_eq s := repeat (step_eq s).
+Ltac tc := try congruence.
+
+Lemma p_eq_body :
+  forall (tbl : parse_table)
+         (sym : symbol)
+         (input : list string)
+         (vis : list nonterminal)
+         (a : Acc triple_lt (meas tbl input vis (F_arg sym))),
+    p tbl sym input vis a =
+    match (sym, input) with
+    | (T _, nil) => (None, input)
+    | (T y, token :: input') =>
+      if beqString y token then
+        (Some (Leaf y), input')
+      else
+        (None, input)
+    | (NT x, _) =>
+      match ptlk_dec x (peek input) tbl with
+      | inl _ => (None, input)
+      | inr (exist _ gamma Hlk) =>
+        match List.in_dec NT_as_DT.eq_dec x vis with
+        | left _ => (None, input)
+        | right Hnin => 
+          match pf tbl gamma input (x :: vis) (hole1 _ _ _ _  _ _ _ a Hlk Hnin) with
+          | (None, _) => (None, input)
+          | (Some sts, input') =>
+            (Some (Node x sts), input')
+          end
+        end
+      end
+    end.
+Proof.
+  intros; destruct a; simpl; cr.
+Qed.
+
+Lemma pf_eq_body :
+  forall (tbl : parse_table)
+         (gamma : list symbol)
+         (input : list string)
+         (vis : list nonterminal)
+         (a : Acc triple_lt (meas tbl input vis (G_arg gamma))),
+    pf tbl gamma input vis a =
+    match gamma as g return gamma = g -> _  with
+    | nil => fun _ => (Some nil, input)
+    | sym :: gamma' => fun Hg => 
+                         match p tbl sym input vis (hole2 _ _ _ _ _ a) with
+                         | (None, _) => (None, input)
+                         | (Some lSib, input') =>
+                           match Compare_dec.lt_dec (List.length input') (List.length input) with
+                           | left Hlt =>
+                             match pf tbl gamma' input' [] (hole3 _ _ _ _ _ _ _ a Hlt) with
+                             | (None, _) => (None, input)
+                             | (Some rSibs, input'') =>
+                               (Some (lSib :: rSibs), input'')
+                             end
+                           | right Hnlt =>
+                             match pf tbl gamma' input vis (hole4 _ _ _ _ _ _ a Hg) with
+                             | (None, _) => (None, input)
+                             | (Some rSibs, input'') =>
+                               (Some (lSib :: rSibs), input'')
+                             end
+                           end
+                         end
+    end eq_refl.
+Proof.
+  intros; destruct a; cr.
+Qed.
+
+Lemma p_t_ret_leaf :
+  forall tbl
+         input rem
+         vis
+         y
+         (a : Acc triple_lt (meas tbl input vis (F_arg (T y))))
+         tr,
+    p tbl (T y) input vis a = (Some tr, rem)
+    -> isLeaf tr = true.
+Proof.
+  intros; destruct a; cr; tc.
+  inv H; auto.
+Qed.
+
+Lemma p_nt_ret_node :
+  forall tbl
+         input rem
+         vis
+         x
+         (a : Acc triple_lt (meas tbl input vis (F_arg (NT x))))
+         tr,
+    p tbl (NT x) input vis a = (Some tr, rem)
+    -> isNode tr = true.
+Proof.
+  intros; destruct a; cr; tc.
+  inv H; auto.
+Qed.
+
+Open Scope list_scope.
+
+Lemma l_ident_eq_nil :
+  forall A (xs ys : list A), xs ++ ys = ys -> xs = [].
+Proof.
+  intros.
+  rewrite <- app_nil_l in H.
+  apply app_inv_tail in H; auto.
+Qed.
+
+Lemma input_length_invariant :
+  forall (g   : grammar)
+         (tbl : parse_table),
+    parse_table_for tbl g
+    -> forall (tr        : tree)
+              (sym       : symbol)
+              (input rem : list terminal)
+              (vis       : list nonterminal)
+              (a : Acc triple_lt (meas tbl input vis (F_arg sym))),
+      p tbl sym input vis a = (Some tr, rem)
+      -> List.length rem < List.length input
+         \/ rem = input.
+Proof.
+  intros g tbl Htbl tr.
+  induction tr as [ s
+                  | s f IHpf
+                  |
+                  | tr IHp f IHpf ]
+                    using tree_nested_ind with
+      
+      (Q := fun f =>
+              forall (gamma : list symbol)
+                     (input rem : list string)
+                     (vis : list nonterminal)
+                     (a   : Acc triple_lt (meas tbl input vis (G_arg gamma))),
+                pf tbl gamma input vis a = (Some f, rem)
+                -> List.length rem < List.length input
+                   \/ rem = input); intros; destruct a.
+
+  - destruct sym as [y | x].
+    + cr; tc.
+      inv H; auto.
+    + apply p_nt_ret_node in H; inv H.
+
+  - destruct sym as [y | x].
+    + apply p_t_ret_leaf in H; inv H.
+    + step; tc.
+      step.
+      step; tc.
+      step_eq Hpf.
+      step; tc.
+      inv H.
+      apply IHpf in Hpf; auto.
+
+  - cr; tc.
+    inv H; auto.
+
+  - step; tc.
+    step_eq Hp.
+    step; tc.
+    step.
+    + step_eq Hpf.
+      step; tc.
+      inv H.
+      apply IHp in Hp; clear IHp.
+      apply IHpf in Hpf; clear IHpf.
+      destruct Hpf.
+      * left; omega.
+      * subst; auto.
+    + step_eq Hpf.
+      step; tc.
+      inv H.
+      apply IHpf in Hpf; clear IHpf.
+      auto.
+Qed.
+          
+Lemma p_sound' :
+  forall (g   : grammar)
+         (tbl : parse_table),
+    parse_table_for tbl g
+    -> forall (tr        : tree)
+              (sym       : symbol)
+              (input rem : list terminal)
+              (vis       : list nonterminal)
+              (a : Acc triple_lt (meas tbl input vis (F_arg sym))),
+      p tbl sym input vis a = (Some tr, rem)
+      -> exists word,
+        word ++ rem = input
+        /\ (@sym_derives_prefix g) sym word tr rem.
+Proof.
+  intros g tbl Htbl tr.
+  induction tr as [ s
+                  | s f IHpf
+                  |
+                  | tr IHp f IHpf ]
+                    using tree_nested_ind with
+
+      (Q := fun f =>
+              forall (gamma : list symbol)
+                     (input rem : list string)
+                     (vis : list nonterminal)
+                     (a   : Acc triple_lt (meas tbl input vis (G_arg gamma))),
+                pf tbl gamma input vis a = (Some f, rem)
+                -> exists word,
+                  word ++ rem = input
+                  /\ gamma_derives_prefix gamma word f rem); intros; destruct a.
+
+  - destruct sym as [y | x].
+    + rewrite p_eq_body in H.
+      step; tc.
+      step_eq Hbeq; tc.
+      inv H.
+      eexists; split.
+      * rewrite cons_app_singleton; auto.
+      * rewrite beqSym_eq in Hbeq; subst.
+        constructor; auto.
+    + apply p_nt_ret_node in H; inv H.
+
+  - destruct sym as [y | x].
+    + apply p_t_ret_leaf in H; inv H.
+    + simpl in H.
+      destruct (ptlk_dec x (peek input) tbl) as [| e]; tc.
+      destruct e as [gamma Hlk].
+      step; tc.
+      step_eq Hpf.
+      step; tc.
+      inv H.
+      apply IHpf in Hpf; clear IHpf.
+      destruct Hpf as [word [Happ Hg]]; subst.
+      eexists; split; eauto.
+      apply Htbl in Hlk; destruct Hlk.
+      econstructor; eauto.
+
+  - rewrite pf_eq_body in H.
+    cr; tc.
+    inv H.
+    exists nil; split; auto.
+    constructor.
+
+  - rewrite pf_eq_body in H.
+    step; tc.
+    step_eq Hp.
+    step; tc.
+    step.
+    + step_eq Hpf.
+      step; tc.
+      inv H.
+      apply IHp in Hp; clear IHp.
+      apply IHpf in Hpf; clear IHpf.
+      destruct Hp  as [wpre [Happ Hs]]; subst.
+      destruct Hpf as [wsuf [Happ Hg]]; subst.
+      exists (wpre ++ wsuf); split.
+      * rewrite app_assoc; auto.
+      * constructor; auto.
+    + pose proof Hp as Hp'.
+      eapply input_length_invariant in Hp'; eauto.
+      destruct Hp'; try contradiction.
+      subst.
+      step_eq Hpf.
+      step; tc.
+      inv H.
+      apply IHp in Hp; clear IHp.
+      apply IHpf in Hpf; clear IHpf.
+      destruct Hp as [wpre [Happ Hs]].
+      apply l_ident_eq_nil in Happ; subst.
+      destruct Hpf as [wsuf [Happ Hg]]; subst.
+      exists ([] ++ wsuf); split; auto.
+      constructor; auto.
+Qed.
+
+Lemma p_sound :
+  forall (g   : grammar)
+         (tbl : parse_table),
+    parse_table_for tbl g
+    -> forall (tr        : tree)
+              (sym       : symbol)
+              (word rem  : list terminal)
+              (vis       : list nonterminal)
+              (a : Acc triple_lt (meas tbl (word ++ rem) vis (F_arg sym))),
+      p tbl sym (word ++ rem) vis a = (Some tr, rem)
+      -> (@sym_derives_prefix g) sym word tr rem.
+Proof.
+  intros g tbl Htbl tr sym word rem vis a Hp.
+  pose proof Hp as Hp'.
+  eapply p_sound' in Hp; eauto.
+  destruct Hp as [word' [Happ Hder]].
+  apply app_inv_tail in Happ.
+  subst; auto.
+Qed.
 
 (* next steps :
 
    - more expressive return type (partial parse tree, left-recursive nonterminal, etc.
    - condense two match expressions in parseForest into single expression? 
-   - way to make arguments to recursive calls more syntactically obvious? 
-   - soundness proof
-   - remove previous drafts from code base
-*)
+   - ask about why ptlk_dec is required
+ *)
+
